tests/lean/run/5407.lean
@@ -1,11 +1,11 @@
 /-!
-# Library search should not return invalid tactics
+# Suggestion tactics should not return invalid tactics
 
 https://github.com/leanprover/lean4/issues/5407
 
-The library-search tactics `exact?` and `apply?` should not suggest proof terms that do not
-compile. If such proof terms are generated, these tactics should instead provide users with
-appropriate feedback.
+The "suggestion" tactics `exact?`, `apply?`, `show_term`, and `rw?` should not suggest proof terms
+that do not compile. They should use `expose_names` where possible to render suggestions valid. If
+an invalid proof is generated, these tactics should instead provide users with appropriate feedback.
 -/
 
 /-! Discards unprintable implicit argument to lambda -/
@@ -22,9 +22,9 @@ theorem odd_iff {n : Nat} : Odd n ↔ n % 2 = 1 := by
 
 /--
 error: found a proof, but the corresponding tactic failed:
-  · expose_names; exact odd_iff.mpr h
+  (expose_names; exact odd_iff.mpr h)
 
-It may be possible to correct this proof by adding type annotations or eliminating unnecessary function abstractions.
+It may be possible to correct this proof by adding type annotations, explicitly specifying implicit arguments, or eliminating unnecessary function abstractions.
 -/
 #guard_msgs in
 example {n : Nat} : n % 2 = 1 → Odd n :=
@@ -38,7 +38,7 @@ opaque C : Prop
 axiom imp : A → B → C
 axiom a : A
 axiom b : B
-/-- info: Try this: · expose_names; exact imp h_1 h -/
+/-- info: Try this: (expose_names; exact imp h_1 h) -/
 #guard_msgs in
 example : C := by
   have h : A := a
@@ -51,20 +51,22 @@ inductive EqExplicit {α} : α → α → Prop
   | intro : (a b : α) → a = b → EqExplicit a b
 /--
 error: found a proof, but the corresponding tactic failed:
-  · expose_names; exact EqExplicit.intro (fun f => (fun g x => g x) f) id rfl
+  (expose_names; exact EqExplicit.intro (fun f => (fun g x => g x) f) id rfl)
 
-It may be possible to correct this proof by adding type annotations or eliminating unnecessary function abstractions.
+It may be possible to correct this proof by adding type annotations, explicitly specifying implicit arguments, or eliminating unnecessary function abstractions.
 -/
 #guard_msgs in
 example : EqExplicit (fun (f : α → β) => (fun g x => g x) f) id := by
   exact?
 
+
 /-! Suggests `expose_names` if a name in the syntax contains macro scopes -/
-/-- info: Try this: · expose_names; exact h -/
+/-- info: Try this: (expose_names; exact h) -/
 #guard_msgs in
 example {P : Prop} : P → P := by
   intro
   exact?
+
 
 /-! Does *not* suggest `expose_names` when the inaccessible name is an implicit argument. -/
 opaque D : Nat → Type
@@ -76,6 +78,7 @@ example : (n : Nat) → D n → C := by
   intro x
   exact?
 
+
 /-! `apply?` logs info instead of erroring -/
 opaque E : Prop
 axiom option1 : A → E
@@ -84,11 +87,87 @@ axiom option2 {_ : B} : E
 info: Try this: refine option1 ?_
 ---
 info: found a partial proof, but the corresponding tactic failed:
-  · expose_names; refine option2
+  (expose_names; refine option2)
 
-It may be possible to correct this proof by adding type annotations or eliminating unnecessary function abstractions.
+It may be possible to correct this proof by adding type annotations, explicitly specifying implicit arguments, or eliminating unnecessary function abstractions.
 ---
 warning: declaration uses 'sorry'
 -/
 #guard_msgs in
 example : E := by apply?
+
+
+/-!
+This `apply?` erroneously reports a failure if suggesting tactics with dot-focusing notation instead
+of parenthesized sequencing.
+-/
+opaque R : A → B → Prop
+axiom rImp (b : B) : R a b → R a b
+/--
+info: Try this: (expose_names; refine rImp b ?_)
+---
+warning: declaration uses 'sorry'
+-/
+#guard_msgs in
+example : (b : B) → R a b := by
+  intro
+  apply?
+
+
+/-! `show_term` exhibits the same behavior as `exact?` -/
+/-- info: Try this: (expose_names; exact h) -/
+#guard_msgs in
+example : E → E := by
+  intro
+  show_term assumption
+/--
+error: found a partial proof, but the corresponding tactic failed:
+  (expose_names; refine option2)
+
+It may be possible to correct this proof by adding type annotations, explicitly specifying implicit arguments, or eliminating unnecessary function abstractions.
+-/
+#guard_msgs in
+example : B → E := by
+  intro
+  show_term apply option2
+/-- info: Try this: exact c_of_d d -/
+#guard_msgs in
+example : (n : Nat) → D n → C := by
+  intro _ d
+  show_term apply c_of_d d
+
+/-! `rw?` exhibits the same behavior as above. -/
+namespace Rw
+
+opaque A : Type
+@[instance] axiom inst : Inhabited A
+noncomputable opaque a : A
+
+axiom eq (a' : A) : a = a'
+
+opaque Foo (a a' : A) : Prop
+
+axiom t : Foo a a
+
+/--
+info: Try this: (expose_names; rw [eq a'])
+-- Foo a' a'
+---
+error: unsolved goals
+a'✝ : A
+⊢ Foo a'✝ a'✝
+-/
+#guard_msgs in
+example : (a' : A) → Foo a a' := by
+  intro
+  rw?
+
+
+axiom eq_imp {a' : A} : a = a'
+example : (a' : A) → Foo a a' := by
+  intro
+  -- FIXME: the goal this displays is wrong
+  -- The current `isDefEq` workaround doesn't work, and may also be too slow for `apply?`
+  -- TODO: this is a different output than we get on Lean nightly -- we're not changing anything
+  -- in the parts of the code this commit touches, so it must be upstream? Debug.
+  rw?
